src/dvspec/dafny/dvc_implementation_spec_proof.dfy
@@ -8,36 +8,6 @@ abstract module DVCNode_Implementation_Proofs refines DVCNode_Implementation
 
     export PublicInterface...
         reveals *
-        // provides 
-        //         toDVCNodeState,
-        //         f_resend_attestation_share,
-        //         toDVCNodeStateAndOuputs,
-        //         Outputs,
-        //         getEmptyOuputs,
-        //         f_att_consensus_decided,
-        //         f_serve_attestation_duty,
-        //         f_listen_for_new_imported_blocks,
-        //         f_listen_for_attestation_shares,
-        //         f_next,
-        //         Event
-        // reveals
-        //         DVCNodeState,
-        //         DVCNodeStateAndOuputs
-        // provides
-        //         DVCNode.network,
-        //         DVCNode.att_consensus, 
-        //         DVCNode.bn,
-        //         DVCNode.current_attesation_duty
-    // export reveals *
-    // export 
-    //     provides Types, DVCNode_Implementation_Helpers, DVCNode_Externs
-    //     reveals DVCNode, toDVCNodeState
-    //     provides 
-    //             DVCNode.serve_attestation_duty, 
-    //             DVCNode.att_consensus_decided, 
-    //             DVCNode.listen_for_attestation_duty_shares,
-    //             DVCNode.listen_for_new_imported_blocks,
-    //             DVCNode.resend_attestation_share
 
     function toDVCNodeState(n: DVCNode): DVCNodeState
     reads n, n.bn, n.rs
@@ -175,63 +145,31 @@ abstract module DVCNode_Implementation_Proofs refines DVCNode_Implementation
             ...;
         }
 
-        lemma lll<T, T2>(s: seq<T>, p: T -> bool, f: T -> T2, i: nat)
-        requires |s| > 0
-        requires i <= |s| - 1;
-        requires !p(s[i])
-        ensures
-            var S := set a | a in s[..i] && p(a) :: f(a);
-            var S2  := set a | a in s[..i+1] && p(a) :: f(a); 
-            S == S2       
-        {
-            
-
-            var S := set a | a in s[..i] && p(a) :: f(a);
-            var S2  := set a | a in s[..i+1] && p(a) :: f(a);
-
-            assert S == S2;
-        }
-
-
-
-        // lemma l2(block: BeaconBlock, old_future_att_consensus_instances_already_decided: set<Slot>, old_process: DVCNodeState)
-        // requires                 
-        // var new_att := future_att_consensus_instances_already_decided - old_future_att_consensus_instances_already_decided; 
-        // block.body.state_root in old(bn.state_roots_of_imported_blocks) ==>
-        //     new_att == xxx(process, block, valIndex, i);  
-        // {                
-
-        //         var a := block.body.attestations[i];
-        //         var committee :- bn.get_epoch_committees(block.body.state_root, a.data.index);
-
-                
-        //         if
-        //         // && a.data.slot == process.attestation_duty.slot 
-        //         // && a.data.index == process.attestation_duty.committee_index
-        //         && valIndex.Some?
-        //         && valIndex.v in committee
-        //         && var i:nat :| i < |committee| && committee[i] == valIndex.v;
-        //         && i < |a.aggregation_bits|
-        //         && a.aggregation_bits[i]
-        //         && (current_attesation_duty.isPresent() ==> a.data.slot >= current_attesation_duty.safe_get().slot)
-        //         {
-        //             future_att_consensus_instances_already_decided := future_att_consensus_instances_already_decided + {a.data.slot};
-        //         }
-        //         else
-        //         {
-        //             assert 
-        //                 var new_att := future_att_consensus_instances_already_decided - old(this.future_att_consensus_instances_already_decided); 
-        //                 var process := old(toDVCNodeState(this));
-        //                 block.body.state_root in old(bn.state_roots_of_imported_blocks) ==>
-        //                     new_att == xxx(process, block, valIndex, i);   
-
-        //             assert 
-        //                 var new_att := future_att_consensus_instances_already_decided - old(this.future_att_consensus_instances_already_decided); 
-        //                 var process := old(toDVCNodeState(this));
-        //                 block.body.state_root in old(bn.state_roots_of_imported_blocks) ==>
-        //                     new_att == xxx(process, block, valIndex, i + 1);                                                   
-        //         }            
-        // }
+        // Helper function used when proving the postcondition of method listen_for_new_imported_blocks below
+        function listen_for_new_imported_blocks_helper(
+            process: DVCNodeState,
+            block: BeaconBlock,
+            valIndex: Optional<ValidatorIndex>,
+            i: nat
+        ) : (new_att: set<Slot>)
+        requires i <= |block.body.attestations|
+        requires block.body.state_root in process.bn.state_roots_of_imported_blocks
+        {            
+            set a |
+                    && a in block.body.attestations[..i]
+                    && isMyAttestation(a, process, block, valIndex)
+                    // && a.data.slot == process.attestation_duty.slot 
+                    // && a.data.index == process.attestation_duty.committee_index
+                    // && var committee := bn_get_epoch_committees(process.bn, block.body.state_root, a.data.index);
+                    // && valIndex.Some?
+                    // && valIndex.v in committee
+                    // && var i:nat :| i < |committee| && committee[i] == valIndex.v;
+                    // && i < |a.aggregation_bits|
+                    // && a.aggregation_bits[i]
+                    // && (process.current_attesation_duty.isPresent() ==> a.data.slot >= process.current_attesation_duty.safe_get().slot)
+                ::
+                    a.data.slot
+        }           
 
         method listen_for_new_imported_blocks...
         ensures block.body.state_root in bn.state_roots_of_imported_blocks ==> f_listen_for_new_imported_blocks(old(toDVCNodeState(this)), block) == toDVCNodeStateAndOuputs(this);
@@ -241,7 +179,7 @@ abstract module DVCNode_Implementation_Proofs refines DVCNode_Implementation
                 invariant 0 <= i <= |block.body.attestations|
                 invariant  block.body.state_root in old(bn.state_roots_of_imported_blocks) ==>
                     future_att_consensus_instances_already_decided == 
-                    old(future_att_consensus_instances_already_decided) + xxx(old(toDVCNodeState(this)), block, valIndex, i); 
+                    old(future_att_consensus_instances_already_decided) + listen_for_new_imported_blocks_helper(old(toDVCNodeState(this)), block, valIndex, i); 
                     
                 invariant toDVCNodeState(this) == old(toDVCNodeState(this)).(
                     future_att_consensus_instances_already_decided := toDVCNodeState(this).future_att_consensus_instances_already_decided
@@ -251,131 +189,6 @@ abstract module DVCNode_Implementation_Proofs refines DVCNode_Implementation
 
             }
         }
-
-        // method listen_for_new_imported_blocks...
-        // ensures block.body.state_root in bn.state_roots_of_imported_blocks ==> f_listen_for_new_imported_blocks(old(toDVCNodeState(this)), block) == toDVCNodeStateAndOuputs(this);
-        // {
-        //     var valIndex :- bn.get_validator_index(block.body.state_root, dv_pubkey);
-        //     var i := 0;
-
-        //     while i < |block.body.attestations|
-        //         invariant 0 <= i <= |block.body.attestations|
-        //         invariant 
-        //                         var new_att := future_att_consensus_instances_already_decided - old(this.future_att_consensus_instances_already_decided); 
-        //         block.body.state_root in old(bn.state_roots_of_imported_blocks) ==>
-        //             future_att_consensus_instances_already_decided == old(future_att_consensus_instances_already_decided) + xxx(old(toDVCNodeState(this)), block, valIndex, i); 
-
-        //         invariant current_attesation_duty == old(toDVCNodeState(this)).current_attesation_duty;
-        //         invariant toDVCNodeState(this) == old(toDVCNodeState(this)).(
-        //             future_att_consensus_instances_already_decided := toDVCNodeState(this).future_att_consensus_instances_already_decided
-        //         )
-        //         invariant toDVCNodeStateAndOuputs(this).outputs == getEmptyOuputs();
-        //     {
-        //         var a := block.body.attestations[i];
-        //         var committee :- bn.get_epoch_committees(block.body.state_root, a.data.index);
-                                 
-        //         if
-        //         // && a.data.slot == process.attestation_duty.slot 
-        //         // && a.data.index == process.attestation_duty.committee_index
-        //         && valIndex.Some?
-        //         && valIndex.v in committee
-        //         && var i:nat :| i < |committee| && committee[i] == valIndex.v;
-        //         && i < |a.aggregation_bits|
-        //         && a.aggregation_bits[i]
-        //         && (current_attesation_duty.isPresent() ==> a.data.slot >= current_attesation_duty.safe_get().slot)
-        //         {
-        //             future_att_consensus_instances_already_decided := future_att_consensus_instances_already_decided + {a.data.slot};                     
-        //         }
-
-        //         i := i + 1;
-        //     }                           
-
-        //     if current_attesation_duty.isPresent() && current_attesation_duty.safe_get().slot in future_att_consensus_instances_already_decided
-        //     {
-        //         att_consensus.stop(current_attesation_duty.safe_get().slot);
-        //         check_for_next_queued_duty();
-        //     } 
-
-        //     assert block.body.state_root in bn.state_roots_of_imported_blocks ==> f_listen_for_new_imported_blocks(old(toDVCNodeState(this)), block) == toDVCNodeStateAndOuputs(this);
-        // }        
-
-        // method listen_for_new_imported_blocks...
-        // // ensures block.body.state_root in bn.state_roots_of_imported_blocks ==> f_listen_for_new_imported_blocks(old(toDVCNodeState(this)), block) == toDVCNodeStateAndOuputs(this);
-        // {
-        //     ...;
-
-        //     while...
-        //         invariant 0 <= i <= |block.body.attestations|
-        //         // invariant 
-        //         // var new_att := future_att_consensus_instances_already_decided - old(this.future_att_consensus_instances_already_decided); 
-        //         // var process := old(toDVCNodeState(this));
-        //         // block.body.state_root in old(bn.state_roots_of_imported_blocks) ==>
-        //         //     new_att == 
-        //         //         set a |
-        //         //             && a in block.body.attestations[..i]
-        //         //             // && a.data.slot == process.attestation_duty.slot 
-        //         //             // && a.data.index == process.attestation_duty.committee_index
-        //         //             && var committee := bn_get_epoch_committees(process.bn, block.body.state_root, a.data.index);
-        //         //             && valIndex.Some?
-        //         //             && valIndex.v in committee
-        //         //             && var i:nat :| i < |committee| && committee[i] == valIndex.v;
-        //         //             && i < |a.aggregation_bits|
-        //         //             && a.aggregation_bits[i]
-        //         //             && (process.current_attesation_duty.isPresent() ==> a.data.slot >= process.current_attesation_duty.safe_get().slot)
-        //         //          ::
-        //         //             a.data.slot;
-        //     {
-        //         assume                 
-        //         var new_att := future_att_consensus_instances_already_decided - old(this.future_att_consensus_instances_already_decided); 
-        //         var process := old(toDVCNodeState(this));
-        //         block.body.state_root in old(bn.state_roots_of_imported_blocks) ==>
-        //             new_att == 
-        //                 set a |
-        //                     && a in block.body.attestations[..i]
-        //                     // && a.data.slot == process.attestation_duty.slot 
-        //                     // && a.data.index == process.attestation_duty.committee_index
-        //                     && var committee := bn_get_epoch_committees(process.bn, block.body.state_root, a.data.index);
-        //                     && valIndex.Some?
-        //                     && valIndex.v in committee
-        //                     && var i:nat :| i < |committee| && committee[i] == valIndex.v;
-        //                     && i < |a.aggregation_bits|
-        //                     && a.aggregation_bits[i]
-        //                     && (process.current_attesation_duty.isPresent() ==> a.data.slot >= process.current_attesation_duty.safe_get().slot)
-        //                  ::
-        //                     a.data.slot;                
-        //         ...;
-
-        //         if...
-        //         {
-
-        //             assert                 
-        //             var new_att := future_att_consensus_instances_already_decided - old(this.future_att_consensus_instances_already_decided); 
-        //             var process := old(toDVCNodeState(this));
-        //             block.body.state_root in old(bn.state_roots_of_imported_blocks) ==>
-        //                 new_att == 
-        //                     set a |
-        //                         && a in block.body.attestations[..i]
-        //                         // && a.data.slot == process.attestation_duty.slot 
-        //                         // && a.data.index == process.attestation_duty.committee_index
-        //                         && var committee := bn_get_epoch_committees(process.bn, block.body.state_root, a.data.index);
-        //                         && valIndex.Some?
-        //                         && valIndex.v in committee
-        //                         && var i:nat :| i < |committee| && committee[i] == valIndex.v;
-        //                         && i < |a.aggregation_bits|
-        //                         && a.aggregation_bits[i]
-        //                         && (process.current_attesation_duty.isPresent() ==> a.data.slot >= process.current_attesation_duty.safe_get().slot)
-        //                     ::
-        //                         a.data.slot;                    
-        //             ...;
-        //         }
-        //         else
-        //         {
-  
-        //         }
-        //         ...;
-        //     }
-        //     ...;
-        // }
 
         method resend_attestation_share...
         ensures f_resend_attestation_share(old(toDVCNodeState(this))) == toDVCNodeStateAndOuputs(this)
